src/SDK/CMM/Defs.dfy
@@ -42,6 +42,7 @@ module {:extern "CMMDefs"} CMMDefs {
       modifies Repr
       ensures Valid() && fresh(Repr - old(Repr))
       ensures res.Success? ==> res.value.plaintextDataKey.Some?
+      ensures res.Success? ==> DecryptionMaterialisFromCMM(res.value.plaintextDataKey.get)
   }
 
   // Predicate works arround a known error in Dafny: https://github.com/dafny-lang/dafny/issues/422 
@@ -50,7 +51,19 @@ module {:extern "CMMDefs"} CMMDefs {
   }
 
   predicate {:opaque } EncryptionMaterialsSignatureOpaque(validEncryptionMaterials: Materials.ValidEncryptionMaterials)
-    {
-      true
-    }
+  {
+    true
+  }
+
+  predicate DecryptionMaterialisFromCMM(key: seq<uint8>)
+  {
+    DecryptionMaterialisFromCMMOpaque(key)
+  }
+
+  predicate {:opaque } DecryptionMaterialisFromCMMOpaque(key: seq<uint8>)
+  {
+    true
+  }
+
+
 }
