src/Crypto/AESEncryption.dfy
@@ -13,7 +13,7 @@ module {:extern "AESEncryption"} AESEncryption {
   export
     provides AESDecrypt, AESEncrypt, AESDecryptExtern, AESEncryptExtern, EncryptionSuites, StandardLibrary, 
       UInt, PlaintextDecryptedWithAAD, EncryptionOutputEncryptedWithAAD, CiphertextGeneratedWithPlaintext,
-      EncryptedWithKey
+      EncryptedWithKey, DecryptedWithKey
     reveals EncryptionOutput
 
   datatype EncryptionOutput = EncryptionOutput(cipherText: seq<uint8>, authTag: seq<uint8>)
@@ -25,6 +25,7 @@ module {:extern "AESEncryption"} AESEncryption {
   predicate {:axiom} EncryptionOutputEncryptedWithAAD(ciphertext: EncryptionOutput, aad: seq<uint8>)
   predicate {:axiom} CiphertextGeneratedWithPlaintext (ciphertext: seq<uint8>, plaintext: seq<uint8>)
   predicate {:axiom} EncryptedWithKey(ciphertext: seq<uint8>, key: seq<uint8>)
+  predicate {:axiom} DecryptedWithKey(plaintext: seq<uint8>, key: seq<uint8>)
 
   function method EncryptionOutputFromByteSeq(s: seq<uint8>, encAlg: EncryptionSuites.EncryptionSuite): (encArt: EncryptionOutput)
     requires encAlg.Valid()
@@ -77,7 +78,8 @@ module {:extern "AESEncryption"} AESEncryption {
     requires |iv| == encAlg.ivLen as int
     requires |authTag| == encAlg.tagLen as int
     ensures res.Success? ==> PlaintextDecryptedWithAAD(res.value, aad)
-    ensures res.Success? ==> CiphertextGeneratedWithPlaintext(cipherTxt, res.value) 
+    ensures res.Success? ==> CiphertextGeneratedWithPlaintext(cipherTxt, res.value)
+    ensures res.Success? ==> DecryptedWithKey(res.value, key)
 
   method AESDecrypt(encAlg: EncryptionSuites.EncryptionSuite, key: seq<uint8>, cipherTxt: seq<uint8>, authTag: seq<uint8>, iv: seq<uint8>, aad: seq<uint8>)
       returns (res: Result<seq<uint8>>)
@@ -90,6 +92,7 @@ module {:extern "AESEncryption"} AESEncryption {
     ensures res.Success? ==> |res.value| == |cipherTxt|
     ensures res.Success? ==> PlaintextDecryptedWithAAD(res.value, aad)
     ensures res.Success? ==> CiphertextGeneratedWithPlaintext(cipherTxt, res.value)
+    ensures res.Success? ==> DecryptedWithKey(res.value, key)
     {
       res := AESDecryptExtern(encAlg, key, cipherTxt, authTag, iv, aad);
       if (res.Success? && |cipherTxt| != |res.value|){
